back to verifying

steel/Zeta.Steel.Application.fsti
@@ -9,16 +9,16 @@ module Zeta.Steel.Application
  *      with specs relating it to the high-level model of a Zeta
  *      application
  **)
+open Steel.ST.Util
 open Zeta.Steel.ApplicationTypes
-open Steel.FractionalPermission
-open Steel.Effect
-module A = Zeta.App
+open Zeta.Steel.Util
+module App = Zeta.App
 module Parser = Zeta.Steel.Parser
 module U8 = FStar.UInt8
 module U16 = FStar.UInt16
 module U32 = FStar.UInt32
 module U64 = FStar.UInt64
-module Array = Steel.Array
+module A = Steel.ST.Array
 module M = Zeta.Steel.ThreadStateModel
 module V = Zeta.Steel.VerifierTypes
 open Zeta.Steel.FormatsManual
@@ -34,48 +34,50 @@ open Zeta.Steel.FormatsManual
 *)
 val run_app_function
       (* fid: The id of the function to run *)
-      (fid: A.appfn_id aprm)
+      (fid: App.appfn_id aprm)
       (* The position in the log where the arguments of the function live *)
+      (#log_bytes:Ghost.erased bytes)
       (log_len:U32.t)
       (log_offset:U32.t)
       (args_len:U32.t)
       (log_array:Parser.byte_array {
+        Seq.length log_bytes == U32.v log_len /\
         Parser.len_offset_slice_ok log_array log_len log_offset args_len
        })
       (* The position in the output log in which to write the results, if any *)
+      (#out_bytes: Ghost.erased bytes)
       (out_len:U32.t)
       (out_offset:U32.t)
       (out:Parser.byte_array {
         Parser.len_offset_ok out out_len out_offset
        })
       (* The state of the verifier, with pointers to the store etc. *)
-      (vtls:V.thread_state_t)
+      (#tsm:M.thread_state_model)
+      (t:V.thread_state_t)
   (* if success, returns the number of bytes written in the output log *)
-   : Steel (option U32.t)
-      (V.thread_state_inv vtls `star` (
-       Array.varray log_array `star`
-       Array.varray out)
-       )
-      (fun x ->
-        V.thread_state_inv vtls `star` (
-        Array.varray log_array `star`
-        Array.varray out))
-      (requires fun _ -> True)
-      (ensures fun h0 res h1 ->
-        let out_bytes_initial = Array.asel out h0 in
-        let out_bytes = Array.asel out h1 in
-        let log_bytes = Array.asel log_array h0 in
-        let arg_bytes = Parser.slice log_bytes log_offset args_len in
-        let tsm0 = V.value_of vtls (focus_rmem h0 _) in
-        let tsm1 = V.value_of vtls (focus_rmem h0 _) in
-        let app_payload : runApp_payload =
-            { fid = fid;
-              rest = { len = args_len;
-                       ebytes = arg_bytes } }
-        in
-        Array.asel log_array h0 == Array.asel log_array h1 /\
-        Seq.slice out_bytes_initial 0 (U32.v out_offset)
-          == Seq.slice out_bytes 0 (U32.v out_offset) /\
-        tsm1 == M.runapp tsm0 app_payload /\
-        True //TODO: specify outputs, res etc.
-        )
+   : STT (option U32.t)
+      (V.thread_state_inv t tsm `star`
+       A.pts_to log_array log_bytes `star`
+       A.pts_to out out_bytes)
+      (fun res ->
+        A.pts_to log_array log_bytes `star`
+        (match res with
+         | None ->
+           exists_ (V.thread_state_inv t) `star`
+           exists_ (A.pts_to out)
+         | Some n_out ->
+           exists_ (fun tsm' ->
+           exists_ (fun out_bytes' ->
+            V.thread_state_inv t tsm' `star`
+            A.pts_to out (out_bytes `Seq.append` out_bytes') `star`
+            pure (
+              let arg_bytes = Parser.slice log_bytes log_offset args_len in
+              let app_payload : runApp_payload =
+              { fid = fid;
+                rest = { len = args_len;
+                         ebytes = arg_bytes } }
+              in
+              tsm' == M.runapp tsm app_payload /\
+              out_bytes' == M.bytes_of_app_results (M.delta_app_results tsm tsm') /\
+              U32.v n_out == Seq.length out_bytes')
+            ))))
