steel/Zeta.Steel.Main.fsti
@@ -6,24 +6,21 @@ module U16 = FStar.UInt16
 module U32 = FStar.UInt32
 module U64 = FStar.UInt64
 open Zeta.Steel.FormatsManual
-open Steel.Memory
-open Steel.Effect.Atomic
-open Steel.Effect
-open Steel.Reference
-open Steel.Array
+open Steel.ST.Util
+open Zeta.Steel.Util
+
+module A = Steel.ST.Array
+module G = Steel.ST.GhostReference
+module Lock = Steel.ST.SpinLock
 
 module T = Zeta.Steel.FormatsManual
 module M = Zeta.Steel.ThreadStateModel
-module A = Steel.Array
 module AEH = Zeta.Steel.AggregateEpochHashes
 module V = Zeta.Steel.Verifier
-module Lock = Steel.SpinLock
 module SA = Zeta.SeqAux
 module MR = Steel.MonotonicReference
 #push-options "--ide_id_info_off"
-val thread_state_pts_to (t:V.thread_state_t)
-                        (tsm:M.thread_state_model)
-  : vprop
+
 
 let grows (#a:Type) :Preorder.preorder (erased (Seq.seq a))
   = let open FStar.Seq in
@@ -44,11 +41,10 @@ let thread_inv (t: V.thread_state_t)
                (logref: AEH.log_ref)
                (mlogref: monotonic_log_t)
   : vprop
-  = h_exists (fun (tsm, committed_entries) ->
-       thread_state_pts_to t tsm `star`
-       ghost_pts_to logref AEH.half committed_entries `star`
-       MR.pts_to mlogref AEH.half tsm.M.processed_entries `star`
-       pure (V.committed_prefix tsm.M.processed_entries committed_entries))
+  = exists_ (fun tsm ->
+       V.thread_state_inv t tsm `star`
+       G.pts_to logref half (M.committed_entries tsm) `star`
+       MR.pts_to mlogref half tsm.M.processed_entries)
 
 noeq
 type thread_state (logrefs:AEH.log_refs_t)
@@ -78,10 +74,11 @@ type top_level_state = {
   epoch_hashes: AEH.aggregate_epoch_hashes logrefs;
 }
 
+/// TODO: a fractional permission variant of Steel.ST.Array
 val array_pts_to (#t:Type0)
                  (a:A.array t)
                  (p:Steel.FractionalPermission.perm)
-                 (v:Seq.lseq t (A.length a))
+                 (v:Seq.seq t)
   : vprop
 
 let tid_positions_ok #l #m (all_threads: Seq.seq (thread_state l m))
@@ -92,54 +89,51 @@ let tid_positions_ok #l #m (all_threads: Seq.seq (thread_state l m))
 
 let core_inv (t:top_level_state)
   : vprop
-  = h_exists (fun (perm, v) ->
+  = exists_ (fun perm ->
+    exists_ (fun v ->
       array_pts_to t.all_threads perm v `star`
-      pure (tid_positions_ok v))
+      pure (tid_positions_ok v)))
 
 let initial_inv (t:top_level_state)
   : vprop
   = core_inv t `star`
-    AEH.h_forall (fun (tid:thread_id) ->
-      if Map.contains t.mlogrefs tid
-      then MR.pts_to (Map.sel t.mlogrefs tid) AEH.half Seq.empty
-      else emp)
+    AEH.forall_threads (fun (tid:thread_id) ->
+      MR.pts_to (Map.sel t.mlogrefs tid) half Seq.empty)
 
 // This creates a Zeta instance
 val init (_:unit)
-  : SteelT top_level_state
-    emp
-    initial_inv
+  : STT top_level_state emp initial_inv
 
 val verify_entries (t:top_level_state)
                    (tid:thread_id)
-                   (len: U32.t) (input:A.array U8.t { A.length input == U32.v len })
+                   (#log_bytes:erased bytes) (len: U32.t) (input:A.array U8.t { A.length input == U32.v len })
                    (out_len: U32.t) (output:A.array U8.t { A.length output == U32.v out_len })
-                   (entries:erased (Seq.seq log_entry_base))
-                   (mlogref:monotonic_log_t)
-  : Steel (bool & U32.t & erased (Seq.seq log_entry_base))
+                   (#entries:elog) (mlogref:monotonic_log_t { Map.sel t.mlogrefs tid == mlogref })
+  : STT (option U32.t) //bool & U32.t & erased (Seq.seq log_entry_base))
     (core_inv t `star`
-     A.varray input `star`
-     A.varray output `star`
-     MR.pts_to mlogref AEH.half entries)
+     A.pts_to input log_bytes `star`
+     exists_ (A.pts_to output) `star`
+     MR.pts_to mlogref half entries)
     (fun res ->
       core_inv t `star`
-      A.varray input `star`
-      A.varray output `star`
-      MR.pts_to mlogref AEH.half (let _, _, e = res in e))
-    (requires fun _ ->
-      Map.sel t.mlogrefs tid == mlogref)
-    (ensures fun h0 (b, n, e) h1 ->
-      let out_bytes = A.asel output h1 in
-      if b
-      then match V.spec_parser_log (A.asel input h0) with
-           | Some (entries', _) ->
+      A.pts_to input log_bytes `star`
+      (match res, V.parse_log log_bytes with
+       | None, _ ->
+         exists_ (A.pts_to output) `star`
+         exists_ (MR.pts_to mlogref half)
+
+       | Some _, None ->
+         pure False
+
+       | Some n_out, Some entries' ->
+         exists_ (fun out_bytes ->
+           A.pts_to output out_bytes `star`
+           MR.pts_to mlogref half (entries `Seq.append` entries') `star`
+           pure (
              let tsm0 = M.verify_model (M.init_thread_state_model tid) entries in
              let tsm1 = M.verify_model tsm0 entries' in
-             e == hide (Seq.append entries entries') /\
-             V.serialized_new_app_results tsm0.app_results tsm1.app_results n out_bytes
-           | _ ->
-             True
-      else True)
+             out_bytes == M.bytes_of_app_results (M.delta_app_results tsm0 tsm1) /\
+             U32.v n_out == Seq.length out_bytes))))
 
 let prefix_of (#a:Type) (s0 s1:Seq.seq a)
   : prop
@@ -150,7 +144,7 @@ let prefix_of (#a:Type) (s0 s1:Seq.seq a)
 let snapshot (r:monotonic_log_t) (s:log) =
   MR.witnessed r (fun s' -> prefix_of s s')
 
-let run_threads (logs:(Map.t tid log)) (tid:tid)
+let run_threads (logs:Map.t tid log) (tid:tid)
   : M.thread_state_model
   = M.verify_model (M.init_thread_state_model tid) (Map.sel logs tid)
 
@@ -159,16 +153,17 @@ let tid_logs (a:M.all_logs) (tid:tid) =
 
 val max_certified_epoch (t:top_level_state)
                         (all_logs: erased M.all_logs)
-  : Steel M.epoch_id
+  : ST M.epoch_id
     (core_inv t)
     (fun _ -> core_inv t)
-    (requires fun _ ->
+    (requires
       forall (tid:tid). let lr_i = Map.sel t.mlogrefs tid in
                    snapshot lr_i (tid_logs all_logs tid))
-    (ensures fun _ max _ ->
+    (ensures fun max ->
       forall (eid:M.epoch_id).
          U32.v eid <= U32.v max ==>
          M.epoch_is_certified all_logs eid)
+
 //From this, we should connect back to the semantic
 //proof and show that the entries are sequentially consistent up to eid
 //except for hash collisions
